src/SpecificGen/GF2213_32ReflectiveAddCoordinates.v
@@ -1,0 +1,76 @@
+Require Import Crypto.BaseSystem.
+Require Import Crypto.ModularArithmetic.PrimeFieldTheorems.
+Require Import Crypto.ModularArithmetic.PseudoMersenneBaseParams.
+Require Import Crypto.ModularArithmetic.PseudoMersenneBaseParamProofs.
+Require Import Crypto.ModularArithmetic.ModularBaseSystem.
+Require Import Crypto.ModularArithmetic.ModularBaseSystemProofs.
+Require Import Crypto.ModularArithmetic.ModularBaseSystemOpt.
+Require Export Crypto.SpecificGen.GF2213_32.
+Require Import Crypto.SpecificGen.GF2213_32BoundedCommon.
+Require Import Crypto.Reflection.Reify.
+Require Import Crypto.Reflection.Syntax.
+Require Import Crypto.Reflection.MapInterp.
+Require Import Crypto.Reflection.Z.Interpretations64.
+Require Crypto.Reflection.Z.Interpretations64.Relations.
+Require Import Crypto.Reflection.Z.Interpretations64.RelationsCombinations.
+Require Import Crypto.Reflection.Z.Reify.
+Require Import Crypto.Reflection.Z.Syntax.
+Require Import Crypto.SpecificGen.GF2213_32Reflective.Common.
+Require Import Crypto.SpecificGen.GF2213_32Reflective.Reified.AddCoordinates.
+Require Import Bedrock.Word Crypto.Util.WordUtil.
+Require Import Coq.Lists.List Crypto.Util.ListUtil.
+Require Import Crypto.Tactics.VerdiTactics.
+Require Import Crypto.Util.ZUtil.
+Require Import Crypto.Util.Tuple.
+Require Import Crypto.Util.Tactics.
+Require Import Crypto.Util.LetIn.
+Require Import Crypto.Util.Notations.
+Require Import Crypto.Util.Bool.
+Require Import Crypto.Util.Decidable.
+Require Import Crypto.Algebra.
+Import ListNotations.
+Require Import Coq.ZArith.ZArith Coq.ZArith.Zpower Coq.ZArith.ZArith Coq.ZArith.Znumtheory.
+Local Open Scope Z.
+
+Time Definition radd_coordinates : Expr9_4Op := Eval vm_compute in radd_coordinatesW.
+
+Declare Reduction asm_interp_add_coordinates
+  := cbv beta iota delta
+         [id
+            interp_bexpr interp_uexpr interp_uexpr_FEToWire interp_uexpr_FEToZ interp_uexpr_WireToFE interp_9_4expr
+            radd_coordinates
+            curry_binop_fe2213_32W curry_unop_fe2213_32W curry_unop_wire_digitsW curry_9op_fe2213_32W
+            WordW.interp_op WordW.interp_base_type
+            Z.interp_op Z.interp_base_type
+            Z.Syntax.interp_op Z.Syntax.interp_base_type
+            mapf_interp_flat_type map_interp WordW.interp_base_type MapInterp mapf_interp word64ize rword64ize
+            Interp interp interp_flat_type interpf interpf_step interp_flat_type fst snd].
+Ltac asm_interp_add_coordinates
+  := cbv beta iota delta
+         [id
+            interp_bexpr interp_uexpr interp_uexpr_FEToWire interp_uexpr_FEToZ interp_uexpr_WireToFE interp_9_4expr
+            radd_coordinates
+            curry_binop_fe2213_32W curry_unop_fe2213_32W curry_unop_wire_digitsW curry_9op_fe2213_32W
+            WordW.interp_op WordW.interp_base_type
+            Z.interp_op Z.interp_base_type
+            Z.Syntax.interp_op Z.Syntax.interp_base_type
+            mapf_interp_flat_type map_interp WordW.interp_base_type MapInterp mapf_interp word64ize rword64ize
+            Interp interp interp_flat_type interpf interp_flat_type fst snd].
+
+
+Time Definition interp_radd_coordinates : SpecificGen.GF2213_32BoundedCommon.fe2213_32W
+                                          -> SpecificGen.GF2213_32BoundedCommon.fe2213_32W
+                                          -> SpecificGen.GF2213_32BoundedCommon.fe2213_32W
+                                          -> SpecificGen.GF2213_32BoundedCommon.fe2213_32W
+                                          -> SpecificGen.GF2213_32BoundedCommon.fe2213_32W
+                                          -> SpecificGen.GF2213_32BoundedCommon.fe2213_32W
+                                          -> SpecificGen.GF2213_32BoundedCommon.fe2213_32W
+                                          -> SpecificGen.GF2213_32BoundedCommon.fe2213_32W
+                                          -> SpecificGen.GF2213_32BoundedCommon.fe2213_32W
+                                          -> Tuple.tuple SpecificGen.GF2213_32BoundedCommon.fe2213_32W 4
+  := Eval asm_interp_add_coordinates in interp_9_4expr (rword64ize radd_coordinates).
+(*Print interp_radd_coordinates.*)
+Time Definition interp_radd_coordinates_correct : interp_radd_coordinates = interp_9_4expr radd_coordinates := eq_refl.
+
+Lemma radd_coordinates_correct_and_bounded : op9_4_correct_and_bounded radd_coordinates add_coordinates.
+Proof. exact_no_check radd_coordinatesW_correct_and_bounded. Time Qed.
