src/SpecificGen/GF41417_32BoundedExtendedAddCoordinates.v
@@ -1,0 +1,67 @@
+Require Import Crypto.ModularArithmetic.PrimeFieldTheorems.
+Require Import Crypto.ModularArithmetic.ModularBaseSystem.
+Require Import Crypto.SpecificGen.GF41417_32Bounded.
+Require Import Crypto.SpecificGen.GF41417_32ExtendedAddCoordinates.
+Require Import Crypto.SpecificGen.GF41417_32BoundedAddCoordinates.
+Require Import Crypto.Util.Tuple.
+Require Import Crypto.Util.Tactics.
+
+Lemma fieldwise_eq_extended_add_coordinates_full' twice_d P10 P11 P12 P13 P20 P21 P22 P23
+  : Tuple.fieldwise
+      (n:=4) GF41417_32BoundedCommon.eq
+      (@GF41417_32BoundedAddCoordinates.add_coordinates
+         twice_d P10 P11 P12 P13 P20 P21 P22 P23)
+      (@ExtendedCoordinates.Extended.add_coordinates
+         GF41417_32BoundedCommon.fe41417_32
+         GF41417_32Bounded.add GF41417_32Bounded.sub GF41417_32Bounded.mul twice_d
+         (P10, P11, P12, P13) (P20, P21, P22, P23)).
+Proof.
+  unfold GF41417_32BoundedCommon.eq.
+  apply -> (fieldwise_map_iff (n:=4) eq GF41417_32BoundedCommon.proj1_fe41417_32 GF41417_32BoundedCommon.proj1_fe41417_32).
+  rewrite add_coordinates_correct.
+  cbv [AddCoordinates.add_coordinates].
+  setoid_rewrite <- fieldwise_eq_edwards_extended_add_coordinates_carry_nocarry.
+  unfold edwards_extended_carry_add_coordinates.
+  match goal with |- ?R ?x ?y => rewrite <- (Tuple.map_id (n:=4) x) end.
+  apply <- (fieldwise_map_iff (n:=4) eq (fun x => x) GF41417_32BoundedCommon.proj1_fe41417_32).
+  apply ExtendedCoordinates.Extended.add_coordinates_respectful_hetero;
+    intros;
+    repeat match goal with
+           | [ |- context[add _ _] ]
+             => rewrite add_correct
+           | [ |- context[sub _ _] ]
+             => rewrite sub_correct
+           | [ |- context[mul _ _] ]
+             => rewrite mul_correct
+           | _ => progress unfold Tuple.fieldwise, Tuple.fieldwise', fst, snd, eq in *
+           | [ |- and _ _ ] => split
+           | [ |- ?x = ?x ] => reflexivity
+           | _ => progress rewrite_strat topdown hints edwards_extended_add_coordinates_correct
+           | _ => congruence
+           end.
+Qed.
+
+Definition add_coordinates' twice_d P1 P2
+  := let '(P10, P11, P12, P13) := P1 in
+     let '(P20, P21, P22, P23) := P2 in
+     @GF41417_32BoundedAddCoordinates.add_coordinates
+       twice_d P10 P11 P12 P13 P20 P21 P22 P23.
+
+Definition add_coordinates twice_d P1 P2
+  := Eval cbv beta iota delta [GF41417_32BoundedAddCoordinates.add_coordinates HList.mapt HList.mapt'] in
+      let '(P10, P11, P12, P13) := P1 in
+      let '(P20, P21, P22, P23) := P2 in
+      @GF41417_32BoundedAddCoordinates.add_coordinates
+        twice_d P10 P11 P12 P13 P20 P21 P22 P23.
+
+Lemma add_coordinates_correct_full twice_d P1 P2
+  : Tuple.fieldwise
+      GF41417_32BoundedCommon.eq
+      (add_coordinates twice_d P1 P2)
+      (@ExtendedCoordinates.Extended.add_coordinates
+         GF41417_32BoundedCommon.fe41417_32
+         GF41417_32Bounded.add GF41417_32Bounded.sub GF41417_32Bounded.mul twice_d P1 P2).
+Proof.
+  destruct_head' prod.
+  rewrite <- fieldwise_eq_extended_add_coordinates_full'; reflexivity.
+Qed.
