src/SpecificGen/GF5211_32BoundedAddCoordinates.v
@@ -1,0 +1,77 @@
+Require Import Coq.ZArith.ZArith.
+Require Import Crypto.SpecificGen.GF5211_32.
+Require Import Crypto.SpecificGen.GF5211_32BoundedCommon.
+Require Import Crypto.SpecificGen.GF5211_32ReflectiveAddCoordinates.
+Require Import Crypto.Util.LetIn.
+Local Open Scope Z.
+
+Local Ltac bounded_t opW blem :=
+  apply blem; apply is_bounded_proj1_fe5211_32.
+
+Local Ltac define_binop f g opW blem :=
+  refine (exist_fe5211_32W (opW (proj1_fe5211_32W f) (proj1_fe5211_32W g)) _);
+  abstract bounded_t opW blem.
+
+Local Opaque Let_In.
+Local Opaque Z.add Z.sub Z.mul Z.shiftl Z.shiftr Z.land Z.lor Z.eqb NToWord64.
+Local Arguments interp_radd_coordinates / _ _ _ _ _ _ _ _ _.
+Definition add_coordinatesW (x0 x1 x2 x3 x4 x5 x6 x7 x8 : fe5211_32W) : Tuple.tuple fe5211_32W 4
+  := Eval simpl in interp_radd_coordinates x0 x1 x2 x3 x4 x5 x6 x7 x8.
+
+Local Ltac port_correct_and_bounded pre_rewrite opW interp_rop rop_cb :=
+  change opW with (interp_rop);
+  rewrite pre_rewrite;
+  intros; apply rop_cb; assumption.
+
+Lemma add_coordinatesW_correct_and_bounded : i9top_correct_and_bounded 4 add_coordinatesW Reified.AddCoordinates.add_coordinates.
+Proof. port_correct_and_bounded interp_radd_coordinates_correct add_coordinatesW interp_radd_coordinates radd_coordinates_correct_and_bounded. Qed.
+
+Local Ltac define_9_4op x0 x1 x2 x3 x4 x5 x6 x7 x8 opW blem :=
+  refine (let ts := opW (proj1_fe5211_32W x0)
+                        (proj1_fe5211_32W x1)
+                        (proj1_fe5211_32W x2)
+                        (proj1_fe5211_32W x3)
+                        (proj1_fe5211_32W x4)
+                        (proj1_fe5211_32W x5)
+                        (proj1_fe5211_32W x6)
+                        (proj1_fe5211_32W x7)
+                        (proj1_fe5211_32W x8) in
+          HList.mapt exist_fe5211_32W (ts:=ts) _);
+  abstract (
+      rewrite <- (HList.hlist_map (F:=fun x => is_bounded x = true) (f:=fe5211_32WToZ));
+      apply add_coordinatesW_correct_and_bounded; apply is_bounded_proj1_fe5211_32
+    ).
+Definition add_coordinates (x0 x1 x2 x3 x4 x5 x6 x7 x8 : fe5211_32) : Tuple.tuple fe5211_32 4.
+Proof. define_9_4op x0 x1 x2 x3 x4 x5 x6 x7 x8 add_coordinatesW add_coordinatesW_correct_and_bounded. Defined.
+
+Local Ltac op_correct_t op opW_correct_and_bounded :=
+  cbv [op];
+  rewrite ?HList.map_mapt;
+  lazymatch goal with
+  | [ |- context[proj1_fe5211_32 (exist_fe5211_32W _ _)] ]
+    => rewrite proj1_fe5211_32_exist_fe5211_32W || setoid_rewrite proj1_fe5211_32_exist_fe5211_32W
+  | [ |- context[proj1_wire_digits (exist_wire_digitsW _ _)] ]
+    => rewrite proj1_wire_digits_exist_wire_digitsW
+  | _ => idtac
+  end;
+  rewrite <- ?HList.map_is_mapt;
+  apply opW_correct_and_bounded;
+  lazymatch goal with
+  | [ |- is_bounded _ = true ]
+    => apply is_bounded_proj1_fe5211_32
+  | [ |- wire_digits_is_bounded _ = true ]
+    => apply is_bounded_proj1_wire_digits
+  end.
+
+Lemma add_coordinates_correct (x0 x1 x2 x3 x4 x5 x6 x7 x8 : fe5211_32)
+  : Tuple.map (n:=4) proj1_fe5211_32 (add_coordinates x0 x1 x2 x3 x4 x5 x6 x7 x8)
+    = Reified.AddCoordinates.add_coordinates (proj1_fe5211_32 x0)
+                                             (proj1_fe5211_32 x1)
+                                             (proj1_fe5211_32 x2)
+                                             (proj1_fe5211_32 x3)
+                                             (proj1_fe5211_32 x4)
+                                             (proj1_fe5211_32 x5)
+                                             (proj1_fe5211_32 x6)
+                                             (proj1_fe5211_32 x7)
+                                             (proj1_fe5211_32 x8).
+Proof. op_correct_t add_coordinates add_coordinatesW_correct_and_bounded. Qed.
